rename spc & Spc to sp & Sp

apc/APCA.v
@@ -10,26 +10,26 @@ Module APCA. Section APCA.
 
   Definition scopes := ["APC"].
 
-  Definition apc_body SpcPure : Ord.t → itree hmodE () :=
-    λ dep_ord, APC dep_ord SpcPure.
+  Definition apc_body SpPure : Ord.t → itree hmodE () :=
+    λ dep_ord, APC dep_ord SpPure.
 
   Definition apc_spec : fspec :=
     mk_fspec (λ (o: Ord.t) varg arg, ⌜varg = o↑ ∧ arg = varg⌝)%I
              (λ _ _ _, True)%I.
 
-  Definition Spc : alist string fspec :=
+  Definition Sp : alist string fspec :=
     Seal.sealing CRIS
       [(APCHdr.apc, apc_spec)].
   
-  Lemma Spc_nodup : List.NoDup (List.map fst Spc).
-  Proof using. unfold Spc. unseal CRIS. prove_nodup. Qed.
+  Lemma Sp_nodup : List.NoDup (List.map fst Sp).
+  Proof using. unfold Sp. unseal CRIS. prove_nodup. Qed.
 
-  Definition fnsems SpcPure :=
-    [(APCHdr.apc, (scopes, mk_specbody apc_spec (cfunN (apc_body SpcPure))))].
+  Definition fnsems SpPure :=
+    [(APCHdr.apc, (scopes, mk_specbody apc_spec (cfunN (apc_body SpPure))))].
 
-  Program Definition Mod SpcPure : SMod.t := {|
+  Program Definition Mod SpPure : SMod.t := {|
     SMod.scopes := scopes;
-    SMod.fnsems := fnsems SpcPure;
+    SMod.fnsems := fnsems SpPure;
     SMod.initial_st := [];
   |}.
   Solve All Obligations with prove_scope.
@@ -37,5 +37,5 @@ Module APCA. Section APCA.
 
   Definition InitCond : iProp Σ := emp%I.
 
-  Definition t u SpcPure Spc := Seal.sealing CRIS (SMod.to_hmod (wsim_ginv u ⊤) Spc (Mod SpcPure)).
+  Definition t u SpPure Sp := Seal.sealing CRIS (SMod.to_hmod (wsim_ginv u ⊤) Sp (Mod SpPure)).
 End APCA. End APCA.
