imp_system/mem/MemIAproof.v
@@ -226,8 +226,8 @@ Module MemIA. Section MemIA.
   Context (csl : string → bool).
   Context (genv : GEnv.t).
   Context (u_s : univ_id).
-  Context (spc : string → option fspec).
-  Context (MemInSpcMem: spc_incl MemA.spc spc).
+  Context (sp : string → option fspec).
+  Context (MemInSpMem: sp_incl MemA.sp sp).
 
   Definition Ist: nat -> alist key Any.t -> alist key Any.t -> iProp Σ :=
     fun _ st_src st_tgt =>
@@ -240,12 +240,12 @@ Module MemIA. Section MemIA.
         (own base_γ ((● (memk_src : _memRA)): memRA))
       ))%I.
 
-  Local Definition MemA := (MemA.t u_s spc).
+  Local Definition MemA := (MemA.t u_s sp).
   Local Definition MemI := (MemI.t csl genv).
   Local Definition IstFull := (IstProd (IstSB MemA.(HMod.scopes) Ist) IstEq).
 
   Lemma simF_alloc : HSim.sim_fun open MemA MemI IstFull MemHdr.alloc.
-  Proof using MemInSpcMem.
+  Proof using MemInSpMem.
     init_simF u_s 0.
     steps_l.
     iDestruct "ASM" as "(% & %)". des; subst; hss.
@@ -289,7 +289,7 @@ Module MemIA. Section MemIA.
   Qed.
 
   Lemma simF_free : HSim.sim_fun open MemA MemI IstFull MemHdr.free.
-  Proof using MemInSpcMem.
+  Proof using MemInSpMem.
     init_simF u_s 0.
   
     steps_l. iDestruct "ASM" as "((% & % & P) & %)". des; subst; hss.
@@ -377,7 +377,7 @@ Module MemIA. Section MemIA.
   Qed.
 
   Lemma simF_load : HSim.sim_fun open MemA MemI IstFull MemHdr.load.
-  Proof using MemInSpcMem.
+  Proof using MemInSpMem.
     init_simF u_s 0.
 
     steps_l. iDestruct "ASM" as "([% P] & %)". subst; hss.
@@ -411,7 +411,7 @@ Module MemIA. Section MemIA.
   Qed.
 
   Lemma simF_store : HSim.sim_fun open MemA MemI IstFull MemHdr.store.
-  Proof using MemInSpcMem.
+  Proof using MemInSpMem.
     init_simF u_s 0.
 
     steps_l. iDestruct "ASM" as "((% & % & P) & %)". subst; hss.
@@ -521,7 +521,7 @@ Module MemIA. Section MemIA.
   Qed.
 
   Lemma simF_cmp : HSim.sim_fun open MemA MemI IstFull MemHdr.cmp.
-  Proof using MemInSpcMem.
+  Proof using MemInSpMem.
     init_simF u_s 0.
     
     steps_l. destruct q. destruct x.
@@ -709,7 +709,7 @@ Module MemIA. Section MemIA.
   Qed.
 
   Lemma simF_cas : HSim.sim_fun open MemA MemI IstFull MemHdr.cas.
-  Proof using MemInSpcMem.
+  Proof using MemInSpMem.
     init_simF u_s 0.
 
     steps_l.
@@ -836,7 +836,7 @@ Module MemIA. Section MemIA.
   Qed.
 
   Theorem sim : HSim.t open MemA MemI (MemA.init_cond csl genv) IstFull.
-  Proof using MemInSpcMem.
+  Proof using MemInSpMem.
     init_sim.
     - rewrite /IstFull /MemA /MemI. unfold_hmod. s.
       iIntros "P". iExists [], [_], [], []. repeat iSplit; et. et. { iPureIntro. ss. }
@@ -860,10 +860,10 @@ Section ctxr.
   Context `{!invG α Σ Γ, !subG Γ Σ, !sinvG Σ Γ α β τ}.
   Context `{!memGΓ Γ}.
 
-  Theorem ctxr csl genv (u_s: univ_id) (spc : string → option fspec)
-      (MemInSpcMem: spc_incl MemA.spc spc) :
+  Theorem ctxr csl genv (u_s: univ_id) (sp : string → option fspec)
+      (MemInSpMem: sp_incl MemA.sp sp) :
     ctx_refines
-      (MemA.t u_s spc, MemA.init_cond csl genv)
+      (MemA.t u_s sp, MemA.init_cond csl genv)
       (MemI.t csl genv, emp%I).
   Proof using. eapply main_adequacy, sim; eauto. Qed.
 End ctxr. End MemIA.
