theories/cancellation/CancelSpawn.v
@@ -15,7 +15,7 @@ Lemma cancel_aux_spawn `{Σ: GRA} md
   (LEN: List.length srcs = Datatypes.length tgts)
   (RET: ∀ vret ret : Any.t, cid = 0 → Q meta vret ret ⊢ ⌜vret = ret⌝)
   (RELS: ∀ k x y, cid ≠ k → srcs !! k = Some x → tgts !! k = Some y → thread_rel md ginv cid k x y)
-  (STB: spc_from md fn = Some f)
+  (STB: sp_from md fn = Some f)
   (KTR: ∀ tid, upaco3 (@elim_rel_def _ md ginv _) bot3 l (ktrS tid) (ktrT tid))
   (SRC : srcs !! cid = Some (Ret ();;; interp_hp (x <- SpawnCancelE fn args;; ktrS x)))
   (TGT : tgts !! cid = Some (Ret ();;; interp_hp (cancel_term md ginv meta Q (x <- HoareSpawnE ginv f fn args;; ktrT x))))
@@ -56,7 +56,7 @@ Proof.
   end.
   iterT 2.
   iterL. tau 1. ls.
-  hexploit spc_in_alist_find; eauto. i. des.
+  hexploit sp_in_alist_find; eauto. i. des.
   reveal ITREE.
   rewrite !alist_find_map_snd !H. s.
   erewrite wrap_elimI_well_scoped; cycle 1.
